sitpn2hvhdl/Soundness.v
@@ -1,6 +1,32 @@
 (** * Semantic Preservation Theorem *)
 
+Require Import GlobalTypes.
+
+(* SITPN Libraries *)
+
+Require Import SitpnTypes.
+Require Import Sitpn.
+Require Import dp.SitpnSemantics.
+
+(* H-VHDL Libraries *)
+
+Require Import HVhdlTypes.
+Require Import Environment.
+Require Import SemanticalDomains.
+Require Import Simulation.
+Require Import SimulationFacts.
+Require Import DesignElaboration.
+Require Import AbstractSyntax.
+Require Import HilecopDesignStore.
+Require Import Initialization.
+
+(* SITPN to H-VHDL Libraries *)
+
 Require Import GenerateHVhdl.
+
+(* Specific Tactics. *)
+
+Require Import Coq.Program.Equality.
 
 (** Defines the relation stating that an SITPN execution environment
     and a H-VHDL design execution environment described the same
@@ -13,9 +39,103 @@ Require Import GenerateHVhdl.
     ports of design [d] that implements the conditions of [sitpn].
 *)
 
-Definition sim_env () := term.
+Definition EnvEq sitpn (Ec : nat -> C sitpn -> bool) (Ep : nat -> Clk -> IdMap value) : Prop := True.
+
+(** Defines the state similarity relation between an SITPN state and
+    a H-VHDL design state.
+ *)
+
+Definition SimState {sitpn} (s : SitpnState sitpn) (dstate : DState) : Prop := False.
+
+(** ** Simulation Lemma *)
+
+Lemma simulation_lemma :
+  forall sitpn Ec s1 s2 tau,
+
+    (* From state s1 to state s2 after tau execution cycles. *)
+    SitpnExecute Ec s1 tau s2 ->
+
+    forall  Mg d Ep dstate1 dstate2 ed dstate mm,
+      
+    (* sitpn translates into d. *)
+    sitpn_to_hvhdl sitpn mm = Success d ->
+
+    (* Environments are similar. *)
+    EnvEq sitpn Ec Ep ->
+
+    (* ed, dstate are the results of the elaboration of d. *)
+    edesign hdstore Mg d ed dstate ->
+
+    (* States s1 and dstate1 are similar; *)
+    SimState s1 dstate1 ->
+    
+    (* From dstate1 to dstate2 after tau execution cycles. *)
+    simloop Ep ed dstate1 (get_behavior d) tau dstate2 ->
+
+    (* Conclusion *)
+    SimState s2 dstate2.
+Proof.
+  intros *; intros Hexec; dependent induction Hexec;
+    intros *; intros Htransl Henveq Helab Hsimstate Hsim.
+  
+  (* CASE tau = 0, trivial. *)
+  - apply simloop_eqstate_at_0 in Hsim; rewrite <- Hsim; assumption.
+
+  (* CASE tau > 0 *)
+  -
+    (* Adds premises of simloop relation in the context (using a lemma
+       instead of inversion). *)
+    match goal with
+    | [ H: tau > 0 |- _ ] => 
+      specialize (simloop_tau_gt0 Ep ed dstate1 (get_behavior d) dstate2 tau H Hsim) as Hex;
+        inversion_clear Hex as (dstate' & Hcyc & Hsim')
+    end.
+
+    (* Specializes the induction hypothesis, then apply the step lemma. *)
+    specialize (IHHexec Mg d Ep dstate' dstate2 ed dstate mm Htransl Henveq Helab).
+    
+Admitted.
+
+(** ** Equal Initial States  *)
+
+Lemma init_states_sim :
+  forall sitpn mm d Mg ed dstate dstate0,
+    
+    (* sitpn translates into d. *)
+    sitpn_to_hvhdl sitpn mm = Success d ->
+
+    (* ed, dstate are the results of the elaboration of d. *)
+    edesign hdstore Mg d ed dstate ->
+
+    (* initialization d's state. *)
+    init ed dstate (get_behavior d) dstate0 ->
+
+    (* init states are similar *)
+    SimState (s0 sitpn) dstate0.
+Proof.
+Admitted.
+  
+(** ** Semantic Preservation Theorem *)
 
 Theorem sitpn2vhdl_sound :
-  forall sitpn d tau Ep Ec dimen s dstate mm,
+  forall sitpn Ec tau s d Mg Ep dstate mm,
+
+    (* sitpn translates into d. *)
     sitpn_to_hvhdl sitpn mm = Success d ->
-.
+
+    (* Environments are similar. *)
+    EnvEq sitpn Ec Ep ->      
+
+    (* sitpn is in state s after tau execution cycles. *)
+    SitpnExecute Ec (s0 sitpn) tau s ->
+    
+    (* d is in state dstate after tau execution cycles. *)
+    simwf hdstore Mg Ep tau d dstate ->
+
+    (* ** Conclusion: final states are equal. ** *)
+    SimState s dstate.
+Proof.
+  inversion_clear 4.
+  specialize (init_states_sim sitpn mm d Mg ed dstate0 dstate1 H H3 H4) as Hinit_eq.
+  apply (simulation_lemma sitpn d Ep Ec Mg (s0 sitpn) s dstate1 dstate ed dstate0 tau mm H H0 H3 Hinit_eq H1 H5).
+Qed.
