hvhdl/HilecopDesignStore.v
@@ -1,0 +1,14 @@
+(** * HILECOP Design Declaration Store  *)
+
+Require Import HVhdlTypes.
+Require Import AbstractSyntax.
+Require Import Petri.
+Require Import Place.
+Require Import Transition.
+
+(** Declares the HILECOP global declaration store containing the
+    declarations of the place and transition designs.  *)
+
+Definition hdstore : IdMap design :=
+  (add transition_entid transition_design
+       (add place_entid place_design (NatMap.empty design))).
